chkpt proof checking specs

src/program_proof/chat/merkle/merkle.v
@@ -12,6 +12,7 @@ Record t :=
 
 Section local_defs.
 Context `{!heapGS Σ}.
+(* TODO: change this with golang change. *)
 Definition own ptr arg : iProp Σ :=
   ∃ sl_B,
   "HB" ∷ own_slice_small sl_B byteT 1 arg.(B) ∗
@@ -37,27 +38,42 @@ Definition encodesF (arg:t) : list u8 :=
   arg.(B).
 End Val.
 
-Section tree.
+Section node.
 Context `{!heapGS Σ}.
 
 (* TODO: will need to carry some invariant that the # of children == 256. *)
 Inductive tree : Type :=
+  (* Cut only exists for proof checking trees. *)
+  | Cut : list u8 → tree
+  | Empty : tree
   | Leaf : list u8 → tree
-  | Interior : list (option tree) → tree.
+  | Interior : list tree → tree.
+
+Fixpoint contains (t : tree) (id : list u8) (val : option (list u8)) : Prop :=
+  match t with
+  | Cut _ => False
+  | Empty => id = [] ∧ val = None
+  | Leaf val' => id = [] ∧ val = (Some val')
+  | Interior children =>
+    match id with
+    | [] => False
+    | pos :: rest =>
+      ∃ child, children !! int.nat pos = Some child ∧ contains child rest val
+    end
+  end.
 
 Definition tree_to_map (t : tree) : gmap (list u8) (list u8) :=
   let fix traverse (t : tree) (acc : gmap (list u8) (list u8)) (path : list u8) :=
     match t with
+    | Cut _ => acc
+    | Empty => acc
     | Leaf val => <[path:=val]>acc
     | Interior children =>
       (* Grab all entries from the children, storing the ongoing path. *)
       (foldr
-        (λ child (p:(Z * gmap (list u8) (list u8))),
-          let acc' := match child with
-                      | None => acc
-                      | Some t' => traverse t' p.2 (path ++ [U8 p.1])
-                      end
-          in (p.1 + 1, acc'))
+        (λ child (pIdxAcc:(Z * gmap (list u8) (list u8))),
+          let acc' := traverse child pIdxAcc.2 (path ++ [U8 pIdxAcc.1])
+          in (pIdxAcc.1 + 1, acc'))
         (0, acc) children
       ).2
     end
@@ -69,15 +85,14 @@ Definition is_nil_hash h : iProp Σ :=
 Definition is_tree_hash' (recur : tree -d> list u8 -d> iPropO Σ) : tree -d> list u8 -d> iPropO Σ :=
   (λ t h,
   match t with
-  | Leaf val => is_hash val h
+  | Cut h' => ⌜h = h'⌝
+  | Empty => is_hash [U8 0] h
+  | Leaf val => is_hash (val ++ [U8 1]) h
   | Interior children =>
       ∃ (child_hashes : list (list u8)),
-      ([∗ list] child;hash ∈ children;child_hashes,
-        match child with
-        | None => is_nil_hash hash
-        | Some t' => ▷ recur t' hash
-        end) ∗
-      is_hash (concat child_hashes) h
+      ([∗ list] child;h2 ∈ children;child_hashes,
+        ▷ recur child h2) ∗
+      is_hash (concat child_hashes ++ [U8 2]) h
   end)%I.
 
 Local Instance is_tree_hash'_contractive : Contractive is_tree_hash'.
@@ -85,9 +100,15 @@ Proof. solve_contractive. Qed.
 
 Definition is_tree_hash : tree → list u8 → iProp Σ := fixpoint is_tree_hash'.
 
-Definition own_tree' (recur : loc -d> tree -d> iPropO Σ) : loc -d> tree -d> iPropO Σ :=
+Definition own_Node' (recur : loc -d> tree -d> iPropO Σ) : loc -d> tree -d> iPropO Σ :=
   (λ ptr arg,
     match arg with
+    (* We should never have cuts in in-memory trees. *)
+    | Cut _ => False
+    | Empty =>
+      ∃ hash,
+      "#His_hash" ∷ is_tree_hash arg hash ∗
+      "%Hnil" ∷ ⌜ptr = null⌝
     | Leaf val =>
       ∃ ptr_v v hash sl_hash sl_children,
       "Hval" ∷ Val.own ptr_v v ∗
@@ -106,64 +127,37 @@ Definition own_tree' (recur : loc -d> tree -d> iPropO Σ) : loc -d> tree -d> iPr
       "Hptr_children" ∷ ptr ↦[Node :: "Children"] (slice_val sl_children) ∗
       "Hchildren" ∷
         ([∗ list] child;ptr_child ∈ children;ptr_children,
-          match child with
-          | None => ⌜ptr_child = null⌝
-          | Some t' => ▷ recur ptr_child t'
-          end)
+          ▷ recur ptr_child child)
     end)%I.
 
-Local Instance own_tree'_contractive : Contractive own_tree'.
+Local Instance own_Node'_contractive : Contractive own_Node'.
 Proof. solve_contractive. Qed.
 
-Definition own_tree : loc → tree → iProp Σ := fixpoint own_tree'.
+Definition own_Node : loc → tree → iProp Σ := fixpoint own_Node'.
 
-Lemma own_tree_unfold ptr arg :
-  own_tree ptr arg ⊣⊢
-  match arg with
-  | Leaf val =>
-    ∃ ptr_v v hash sl_hash sl_children,
-    "Hval" ∷ Val.own ptr_v v ∗
-    "Hptr_val" ∷ ptr ↦[Node :: "Val"] #ptr_v ∗
-    "#His_hash" ∷ is_tree_hash arg hash ∗
-    "Hhash" ∷ own_slice_small sl_hash byteT 1 hash ∗
-    "Hsl_hash" ∷ ptr ↦[Node :: "hash"] (slice_val sl_hash) ∗
-    "Hchildren" ∷ own_slice_small sl_children ptrT 1 (replicate 256 null) ∗
-    "Hsl_children" ∷ ptr ↦[Node :: "Children"] (slice_val sl_children)
-  | Interior children =>
-    ∃ hash sl_hash sl_children ptr_children,
-    "Hptr_val" ∷ ptr ↦[Node :: "Val"] #null ∗
-    "#His_hash" ∷ is_tree_hash arg hash ∗
-    "Hhash" ∷ own_slice_small sl_hash byteT 1 hash ∗
-    "Hsl_children" ∷ own_slice_small sl_children ptrT 1 ptr_children ∗
-    "Hptr_children" ∷ ptr ↦[Node :: "Children"] (slice_val sl_children) ∗
-    "Hchildren" ∷
-      ([∗ list] child;ptr_child ∈ children;ptr_children,
-        match child with
-        | None => ⌜ptr_child = null⌝
-        | Some t' => ▷ own_tree ptr_child t'
-        end)
-  end.
-Proof. apply (fixpoint_unfold own_tree'). Qed.
-End tree.
+Lemma own_Node_unfold ptr arg :
+  own_Node ptr arg ⊣⊢ (own_Node' own_Node) ptr arg.
+Proof.
+  apply (fixpoint_unfold own_Node').
+Qed.
 
-Module RootedTree.
-Record t :=
-  mk {
-    Root: tree;
-    PtrRoot: loc;
-  }.
+End node.
 
+Module Tree.
 Section local_defs.
 Context `{!heapGS Σ}.
 Definition own ptr arg : iProp Σ :=
-  "Hroot" ∷ own_tree arg.(PtrRoot) arg.(Root) ∗
-  "Hptr_root" ∷ ptr ↦[Tree :: "Root"] #arg.(PtrRoot).
+  ∃ tree root,
+  "Htree" ∷ own_Node root tree ∗
+  "%Htree_map" ∷ ⌜tree_to_map tree = arg⌝ ∗
+  "Hptr_root" ∷ ptr ↦[Tree :: "Root"] #root.
 End local_defs.
-End RootedTree.
+End Tree.
 
-Section proof.
+Section TreeProofs.
 Context `{!heapGS Σ}.
 
+(*
 Lemma wp_InteriorHash children ptr_tree old_hash sl_children ptr_children :
   {{{
     "Hptr_val" ∷ ptr_tree ↦[Node :: "Val"] #null ∗
@@ -174,13 +168,13 @@ Lemma wp_InteriorHash children ptr_tree old_hash sl_children ptr_children :
       ([∗ list] child;ptr_child ∈ children;ptr_children,
         match child with
         | None => ⌜ptr_child = null⌝
-        | Some t' => ▷ own_tree ptr_child t'
+        | Some t' => ▷ own_Node ptr_child t'
         end)
   }}}
   Node__UpdateInteriorHash #ptr_tree
   {{{
     RET #();
-    own_tree ptr_tree (Interior children)
+    own_Node ptr_tree (Interior children)
   }}}.
 Proof. Admitted.
 
@@ -188,7 +182,7 @@ Lemma sep_nil_children :
  ⊢
  ([∗ list] child;ptr_child ∈ replicate 256 None;replicate (int.nat 256) null,
    match child with
-   | Some t' => ▷ own_tree ptr_child t'
+   | Some t' => ▷ own_Node ptr_child t'
    | None => ⌜ptr_child = null⌝
    end).
 Proof.
@@ -227,4 +221,88 @@ Proof.
   iFrame.
 Qed.
 
-End proof.
+(* TODO: not enough time to write down proof record. *)
+Definition Proof_own (ptr_proof:loc) (proof:u64) : iProp Σ.
+Admitted.
+ *)
+
+(*
+Pre: valid tree at ptr_tree that goes to some map.
+Post: valid tree at ptr_tree that goes to new map.
+ *)
+Lemma wp_Put ptr_tree entry_map ptr_id id ptr_val val :
+  {{{
+    "Htree" ∷ Tree.own ptr_tree entry_map ∗
+    "Hid" ∷ Id.own ptr_id id ∗
+    "Hval" ∷ Val.own ptr_val val
+  }}}
+  Tree__Put #ptr_tree #ptr_id #ptr_val
+  {{{
+    sl_digest ptr_proof (err:u64),
+    RET ((slice_val sl_digest), #ptr_proof, #err);
+    if bool_decide (err = 0) then
+      "Htree" ∷ Tree.own ptr_tree (<[id.(Id.B):=val.(Val.B)]>entry_map)
+    else True%I
+  }}}.
+Proof. Admitted.
+
+(* TODO: all the other tree specs. *)
+
+End TreeProofs.
+
+Module MembProof.
+Section local_defs.
+Context `{!heapGS Σ}.
+Definition own (ptr : loc) : iProp Σ.
+Admitted.
+End local_defs.
+End MembProof.
+
+Module NonmembProof.
+Section local_defs.
+Context `{!heapGS Σ}.
+Definition own (ptr : loc) : iProp Σ.
+Admitted.
+End local_defs.
+End NonmembProof.
+
+Section CheckProofs.
+Context `{!heapGS Σ}.
+
+Definition is_path (id : list u8) (val : option (list u8)) (digest : list u8) : iProp Σ :=
+  ∃ tree,
+  is_tree_hash tree digest ∧
+  ⌜contains tree id val⌝.
+
+Lemma wp_MembCheck ptr_proof ptr_id id ptr_val val sl_dig dig :
+  {{{
+    "Hproof" ∷ MembProof.own ptr_proof ∗
+    "Hid" ∷ Id.own ptr_id id ∗
+    "Hval" ∷ Val.own ptr_val val ∗
+    "Hdig" ∷ own_slice_small sl_dig byteT 1 dig
+  }}}
+  MembProof__Check #ptr_proof #ptr_id #ptr_val (slice_val sl_dig)
+  {{{
+    (err:u64), RET #err;
+    if bool_decide (err = 0) then
+      "Hpath" ∷ is_path (id.(Id.B)) (Some val.(Val.B)) dig
+    else True%I
+  }}}.
+Proof. Admitted.
+
+Lemma wp_NonmembCheck ptr_proof ptr_id id sl_dig dig :
+  {{{
+    "Hproof" ∷ MembProof.own ptr_proof ∗
+    "Hid" ∷ Id.own ptr_id id ∗
+    "Hdig" ∷ own_slice_small sl_dig byteT 1 dig
+  }}}
+  MembProof__Check #ptr_proof #ptr_id (slice_val sl_dig)
+  {{{
+    (err:u64), RET #err;
+    if bool_decide (err = 0) then
+      "Hpath" ∷ is_path (id.(Id.B)) None dig
+    else True%I
+  }}}.
+Proof. Admitted.
+
+End CheckProofs.
